# Logic :: Proof methods :: Index :: Proof by contrapositive

https://en.wikipedia.org/wiki/Proof_by_contrapositive

The contrapositive of a conditional statement is formed by negating both terms and reversing the direction of inference, `p -> q` ≡ `¬p <- ¬q`.

`p -> q` ≡ `¬p <- ¬q` ≡ `¬q -> ¬p`

More specifically, the contrapositive of the statement "if A, then B" is "if not B, then not A." A statement and its contrapositive are logically equivalent, in the sense that if the statement is true, then its contrapositive is true and vice versa.
