
https://en.wikipedia.org/wiki/List_of_theorems


$$
\begin{array}{lll}
  1 & x = y    & \textrm{premise} \\
  2 & x^2 = xy & \textrm{multiply by x} \\
  3 & x^2−y^2 = xy − y^2 & \textrm{subtract }y^2 \\
  4 & (x+y)(x−y) = y(x-y) & \textrm{factor out} \\
  5 & x + y = y & \textrm{cancel } (x−y) \\
  6 & y + y = y & \textrm{according to 1, x=y} \\
  7 & 2y = y & \textrm{divide by y} \\
  \hline
  8 & 2 = 1    &  \textrm{conclusion!} \\
\end{array}
$$


| step                      | desc                                   |
|---------------------------|----------------------------------------|
| x = y                     | premise                                |
| x2 = xy                   | multiply both sides by x               |
| x2 − y2 = xy − y2         | subtract y2 from both sides            |
| (x + y)(x − y) = y(x − y) | factor both sides                      |
| x + y = y                 | cancel (x − y)                         |
| y + y = y                 | remembering x = y, from the first line |
| 2y = y                    | divide both sides by y                 |
| 2 = 1                     |                                        |


hidden division by zero (in 5) allows facilitates the incorrect conclusion.

After factoring in line four, it seems convenient and wise to divide by the common factor (x − y) to obtain line five; however, line one tells us that x = y so x−y = 0, and division by zero is not allowed! 
