# ZFC Axioms

## All ZF axioms

1. Axiom of Extensionality:     
  `âˆ€aâŸâˆ€bâŸ(âˆ€xâŸ(x âˆˆ a âŸº x âˆˆ b) âŸº (a = b))`

2. Axiom of Regularity:    
  `âˆ€xâŸ(x â‰  âˆ… -> âˆƒy((y âˆˆ x) â‹€ (y â‹‚ x = âˆ…)))`

3. Axiom Schema of Specification:     
  `âˆ€(wâ‚âŸâ€¦âŸwâ‚™)âŸâˆ€aâŸ(âˆƒbâŸ(âˆ€xâŸ(x âˆˆ b -> (x âˆˆ a â‹€ Ï†(x, wâ‚,âŸâ€¦,âŸwâ‚™, a)))))`

4. Axiom of Pairing:    
  `âˆ€xâŸâˆ€yâŸâˆƒpâŸ((x âˆˆ p â‹€ x âŠ† p) â‹ (y âˆˆ p â‹€ y âŠ† p))`

5. Axiom of Union:    
  `âˆ€ð“•âŸâˆƒaâŸâˆ€yâŸâˆ€xâŸ(x âˆˆ y â‹€ y âˆˆ ð“• -> x âˆˆ a)`

6. Axiom Schema of Replacement:   
  `âˆ€aâŸâˆ€(wâ‚âŸâ€¦âŸwâ‚™)âŸâˆ€xâŸ((x âˆˆ a -> !âˆƒy.Ï•) -> âˆƒbâŸâˆ€xâŸ(x âˆˆ a -> âˆƒyâŸ(y âˆˆ b â‹€ Ï•)))`

7. Axiom of Infinity:   
  `âˆƒxâŸâˆƒeâŸ(âˆ€zâŸ(z âˆ‰ e) â‹€ (e âˆˆ x) â‹€ âˆ€yâŸ(y âˆˆ x -> (Sy âˆˆ x)))`

8. Axiom of Powerset:    
  `âˆ€zâŸâˆ€xâŸ(z âŠ† x -> âˆ€qâŸ(q âˆˆ z -> q âˆˆ x))`

9. Well-Ordering Theorem:   
  `âˆ€xâŸâˆƒRâŸ(R ð™¬ð™šð™¡ð™¡-ð™¤ð™§ð™™ð™šð™§ð™¨ x)`







- [Axiom of extensionality](https://en.wikipedia.org/wiki/Axiom_of_extensionality)
- [Axiom of empty set](https://en.wikipedia.org/wiki/Axiom_of_empty_set)
- [Axiom of pairing](https://en.wikipedia.org/wiki/Axiom_of_pairing)
- [Axiom of union](https://en.wikipedia.org/wiki/Axiom_of_union)
- [Axiom of infinity](https://en.wikipedia.org/wiki/Axiom_of_infinity)
- [Axiom schema of replacement](https://en.wikipedia.org/wiki/Axiom_schema_of_replacement)
- [Axiom of power set](https://en.wikipedia.org/wiki/Axiom_of_power_set)
- [Axiom of regularity](https://en.wikipedia.org/wiki/Axiom_of_regularity)
- [Axiom schema of specification](https://en.wikipedia.org/wiki/Axiom_schema_of_specification)



## Set Theory (Part 2): ZFC Axioms
https://www.youtube.com/watch?v=op3WZRUKk_k

Intro to the axioms of set theory using the Zermelo-Fraenkel with the axiom of choice (ZFC) formal system.

Showing how the union, the intersection, the empty set and the relative complement are derived or defined under this axiomatic system.


## The axiom of extensionality

https://en.wikipedia.org/wiki/Axiom_of_extensionality


`âˆ€aâŸâˆ€bâŸ(âˆ€xâŸ(x âˆˆ a âŸº x âˆˆ b) âŸº (a = b))`


We can arrive to this axiom if we first consider the subset relation:   
âˆ€aâŸâˆ€bâŸ(âˆ€xâŸ(x âˆˆ a -> x âˆˆ b) -> (a âŠ† b))

This relates sets `a` and `b` in that `a` is a subset of `b`, `a âŠ† b`, if all the elements of `a` are also the elements of `b`.

But if this relation holds in both directions, i.e. if `a âŠ† b` and `b âŠ† a`, then it signifies the set equality in that `a` and `b` are, in fact, the same set since they have all the same elements in common.



## The Axiom of pairing

For all sets X and Y, there is a set C which contains them as its elements. Since X and Y are sets, it means that, besides each being a member of C, each one is also a subset of C.

$$
X=\{a,b\} \\
Y=\{c,d\} \\
C=\{X,Y\} = \{ \{a,b\}, \{c,d\} \} \\
$$

$$\forall X\ \forall Y\ \exists C\ . (X \in C \land X \subseteq C) \lor (Y\in C \land Y \subseteq C)$$
