# Common formulae

P1. 0 ∈ ℕ
P2. n ∈ ℕ -> S(n) ∈ ℕ    S(n) is a function (n + 1) ≡ n', not a predicate

> INDUCTION
P n:
1. P 0
2. P n -> P (S n)

P(0) -> ???
P(n) -> P(n+1)





`∀x ∈ ℕ. ℙx` is ∀x.(ℕx -> ℙx)
`∃x ∈ ℕ. ℙx` is `∃x.(ℕx ∧ ℙx)`



## Drinker's paradox
https://en.wikipedia.org/wiki/Drinker_paradox

`∃x.A(x) -> ∀x.A(x)`

"There is someone in the pub such that, if that person is drinking, then everyone in the pub is drinking".
1. confusing formal implication with causation
2. the person the statement holds true for at one instant is not necessarily the same person it holds true for at any other instant.

similar: "If there's a fish called Joe in the aquarium all alone, then all the fish in the aquarium are named Joe".
