# Logarithm

## Logarithm with any base

Change of base: the base `a` of the logarithm of `x` base `a`, `logₐx` can be coverted into a different base `j` by finding the quotient `logⱼ(x) ÷ logⱼ(a)`.
- logₐ(x) = logⱼ(a) ÷ logⱼ(x)
- logₐ(x) = logₑ(a) ÷ logₑ(x) = ln(a) ÷ ln(x)
- ln(a × b) = ln(a) + ln(b)
- ln(a ÷ b) = ln(a) - ln(b)
- ln(e) = 1
- `e ≈ 2.71828182`
- e⁰ = 1
- eᵉ = 15.1542622415


```js
      ∞
     ⎲   xⁿ
eˣ = ⎳ -----
     ⁿ⁼⁰  n!

     ∞
    ⎲   1ⁿ       1     1      1      1
e = ⎳ ----- =  ---- + ---- + ---- + ---- + … = 1 + 1 + 1/2! + 1/3! + 1/4! + …
    ⁿ⁼⁰  n!       0!    1!     2!     3!

e ≈ 1 + 1 + 1/2 + 1/6 + 1/24 + 1/120 + 1/720 + 1/5040 = 2.7182 5396825
e = 2.7182818284…


// log-base-a-of-x as log-base-b quotient
          logⱼ(a)
logₐ(x) = -------
          logⱼ(x)



logₐ(x) = logₑ(a) ÷ logₑ(x) = ln(a) ÷ ln(x) = ln(a-x)




logₐ(x) = ln(x)

ln(x) = logₑ(x)
logₑ(x)
```


## Natural logarithm

logₑ(x) = ln(x)
- eˡⁿ ˣ = x,   e^(ln x) = x
- eᵃᣟˡⁿ ˣ = xᵃ, e^(a ln x) = xᵃ
- ln(eˣ) = x
- ln(a∙eˣ) = x
- ln(eˣ∙eʸ) = x + y
- ln(ab) = ln(a) + ln(b)    `ln` turns mult into addition
- ln(a÷b) = ln(a) - ln(b)   `ln` turns division into subtraction
- eᵃeᵇ = a + b
- (eᵃ)ᵇ = ab
- ln((eᵃ)ᵇ) = ab
- ln(2³) = 3∙ln(2)

Natural logarithm can expres logarithm of any base.
