# Quadratic relation

https://www.youtube.com/playlist?list=PLwExBww6XoLFdS9Wb3mhZXOlFQlXUYMjP


Let me show you how you can recognize a quadratic relation from the 3 ways any relation can be represented:
- from equation: degree 2 polynomial
- from table: constant 2nd differences
- from graph: parabola

(what does he mean by "relation": a proper relation as in a set of ordered pairs, or is he abusing the term "polynomial", or merely an "equation"?)

An example of an equation that involves a quadratic relation between an `x`
and `y` variable is `y = x² - 6x + 8`. This is a quadratic relation because the highest exponent on the variable is two.

Quadratic relations (?) are also known as degree 2 *polinomial equations*.

The table shows values of `x` for the quadratic relation

    a = 1, b = -6, c = 8
    y = ax² - bx + c
    -------------------
    y = x² - 6x + 8
    f(x) = x² - 6x + 8
    f(x) = y

x  | f(x) = x² - 6x + 8                                | rslt| δ  |  Δ | R
---|---------------------------------------------------|-----|----|----|---
 1 | f(1)  =  1² - 6∙1  + 8  =   1 -  6 + 8  =  -5 + 8 |   3 |    |    | (<)
 2 | f(2)  =  2² - 6∙2  + 8  =   4 - 12 + 8  =  -8 + 8 |   0 | -3 |  3 | (<)
 3 | f(3)  =  3² - 6∙3  + 8  =   9 - 18 + 8  =  -8 + 8 |  -1 | -1 |  1 | (<)
 4 | f(4)  =  4² - 6∙4  + 8  =  16 - 24 + 8  =  -8 + 8 |   0 |  1 |  1 | (<)
 5 | f(5)  =  5² - 6∙5  + 8  =  25 - 30 + 8  =  -5 + 8 |   3 | -3 |  3 | (<)
 6 | f(6)  =  6² - 6∙6  + 8  = `36`-`36`+ 8  =   0 + 8 |   8 |  5 |  5 | (==)
 7 | f(7)  =  7² - 6∙7  + 8  =  49 - 42 + 8  =   7 + 8 |  15 |  7 |  7 | (>)
 8 | f(8)  =  8² - 6∙8  + 8  =  64 - 48 + 8  =  16 + 8 |  24 |  9 |  9 | (>)
 9 | f(9)  =  9² - 6∙9  + 8  =  81 - 54 + 8  =  27 + 8 |  35 | 11 | 11 | (>)
10 | f(10) = 10² - 6∙10 + 8  = 100 - 60 + 8  =  40 + 8 |  48 | 13 | 13 | (>)
11 | f(11) = 11² - 6∙11 + 8  = 121 - 66 + 8  =  55 + 8 |  63 | 15 | 15 | (>)
12 | f(12) = 12² - 6∙12 + 8  = 144 - 72 + 8  =  72 + 8 |  80 | 17 | 17 | (>)
13 | f(13) = 13² - 6∙13 + 8  = 169 - 78 + 8  =  91 + 8 |  99 | 19 | 19 | (>)


The polynomial function `g(x) = x² - 6x + 8` is equal to `f(x) = (x - a)² + b`
