# Quadratic equations

```js
ax² + bx + c
(x + m)(x + n)
such that: m + n = b, mn = c
ax² + (m + n)x + mn
d = avg(m,n) = b/2
m = b/2 - w
n = b/2 + w
ax² + ((b/2 - w) + (b/2 + w))x + (b/2 - w)(b/2 + w)
ax² + bx + b²/4 - w²



(x + 1)² = (x + 1)(x + 1) = x² + 2x + 1
(x - 1)² = (x - 1)(x - 1) = x² - 2x + 1

(x + 3)(x + 5) = x² + 5x + 3x + 15 = x² + 8x - 15
(x - 3)(x + 5) = x² + 5x - 3x - 15 = x² + 2x - 15
(x + 3)(x - 5) = x² - 5x + 3x - 15 = x² - 2x - 15
(x - 3)(x - 5) = x² - 5x - 3x - 15 = x² - 8x - 15

(x - 2)(x - 7) = x² - 7x - 2x + 14 = x² - 9x - 14
(x - 2)(x + 7) = x² + 7x - 2x - 14 = x² + 5x - 14
(x + 2)(x - 7) = x² - 7x + 2x - 14 = x² - 5x - 14

x² + 32x + 192 = (x + 24)(x + 8) = x² + 8x + 24x + 192 = x² + 32x + 192
m = 8, n = 24
avg(m,n) = d = 32/2 = 16
16 ± d
16 - 8 = 8
16 + 8 = 24

8 + 8 = 24 - 8
16 - d = m
16 - d = 8
16 - 8 = 8

16 + d = n
16 + d = 24
16 + 8 = 24


8|192
24|192
8+24|192
8⋅24=192


x² + 9x + 20


x² + 8x + 4
x² + 4x + 10
2x² - 7x - 4

x² - 6x - 91
```
